WIP

src/example/ClientSpinlock2.v
@@ -2,10 +2,10 @@ From sflib Require Import sflib.
 From Paco Require Import paco.
 Require Import Coq.Classes.RelationClasses Lia Program.
 From Fairness Require Import pind Axioms ITreeLib Red TRed IRed2 WFLibLarge.
-From Fairness Require Import FairBeh Mod Linking.
-From Fairness Require Import Spinlock.
+From Fairness Require Import FairBeh Mod Concurrency Linking.
 From Fairness Require Import PCM IProp IPM IPropAux.
-From Fairness Require Import IndexedInvariants OpticsInterp SimWeakest.
+From Fairness Require Import IndexedInvariants OpticsInterp SimWeakest SimWeakestAdequacy.
+From Fairness Require Import Spinlock.
 From Fairness Require Import TemporalLogic SCMemSpec SpinlockSpec.
 From Fairness Require Import AuthExclsRA ExclsRA OneShotsRA.
 
@@ -107,12 +107,13 @@ Section SIM.
   Context {HasAuthExcls : @GRA.inG (AuthExcls.t nat) Γ}.
   Context {HasExcls : @GRA.inG (Excls.t unit) Γ}.
 
-  Context {HasOneShots : @GRA.inG (OneShots.t nat) Γ}.
-  Context {HasOneShots2 : @GRA.inG (OneShots.t unit) Γ}.
+  Context {HasOneShotsNat : @GRA.inG (OneShots.t nat) Γ}.
 
   Ltac red_tl_all := red_tl; red_tl_memra; red_tl_authexcls; red_tl_excls; red_tl_oneshots.
 
   Import ClientSpinlock2.
+
+  Local Opaque X D.
 
   (** Invariants. *)
 
@@ -124,10 +125,12 @@ Section SIM.
   Lemma md_N_ClientSpinlock2_Spinlock : (↑N_ClientSpinlock2 : coPset) ## (↑N_Spinlock : coPset).
   Proof. apply ndot_ne_disjoint. ss. Qed.
 
-  Definition ClientSpinlock2_inv n (tid2 : thread_id) (γX γe κs : nat) (κl γκl : nat) (γr : nat) : sProp n :=
+
+  Definition clientSpinlock2_inv n (tid2 : thread_id) (ℓL ℓl : nat) (γX γe κs : nat) (κl γκl : nat) (γr : nat) : sProp n :=
     (
       ((○ γX 0) ∗ (D ↦ 0)
                 ∗ (-[κl](0)-◇ (∃ (γκw : τ{nat}), ▿ γκl γκw)) ∗ (△ γκl (1/2))
+                ∗ ◇[κs](ℓL, 2)
                 ∗ (Duty(tid2) [])
       )
       ∨
@@ -135,32 +138,39 @@ Section SIM.
                   ∗ (∃ (κw γκw : τ{nat}),
                         (-[κw](0)-◇ (∃ (γκu : τ{nat}), ▿ γκw γκu))
                           ∗ (△ γκw (1/2)) ∗ (κw -(0)-◇ κs) ∗ (▿ γκl γκw)
+                          ∗ ◇[κs](ℓL, 1)
                           ∗ (Duty(tid2) []))
         )
       ∨
         ((○ γX 1) ∗ (D ↦ 1)
-                  ∗ (∃ (κw γκw κu γκu : τ{nat}),
-                        (-[κu](0)-◇ (▿ γκu tt))
+                  ∗ (∃ (γκw κu γκu : τ{nat}),
+                        (-[κu](0)-◇ (▿ γκu 0))
                           ∗ (△ γκu (1/2)) ∗ (κu -(0)-◇ κs) ∗ (▿ γκl γκw) ∗ (▿ γκw γκu)
-                          ∗ ((Duty(tid2) [(κu, 0, (▿ γκu tt))] ∗ (EX γe tt)) ∨ (▿ γr tt)))
+                          ∗ ((Duty(tid2) [(κu, 0, (▿ γκu 0))] ∗ ◇[κu](ℓl, 1) ∗ (EX γe tt)) ∨ (▿ γr 0)))
         )
       ∨
         ((○ γX 0) ∗ (D ↦ 1)
-                  ∗ (∃ (κw γκw κu γκu : τ{nat}),
-                        (▿ γκl γκw) ∗ (▿ γκw γκu) ∗ (▿ γr tt) ∗ (▿ γκu tt)))
+                  ∗ (∃ (γκw γκu : τ{nat}),
+                        (▿ γκl γκw) ∗ (▿ γκw γκu) ∗ (▿ γr 0) ∗ (▿ γκu 0)))
     )%S.
 
+  (* Obligation dependencies: (κl at >= (2 + ℓL) + c) → (κw at 2) → (κu at 2 (=ℓl)) → (κs at >= 3) *)
 
   Lemma ClientSpinlock2_thread1_sim
-        tid n
+        tid n tid2
+        ℓL ℓl
+        (LAYER_L : ℓL = 3)
+        (LAYER_l : ℓL = 2)
     :
-    ⊢ ⟦(∀ (γk k : τ{nat, 1+n}),
-           ((⤉ syn_inv n N_Client01 (client01Inv γk k n))
+    ⊢ ⟦(∀ (γX γe κs κl γκl γr : τ{nat, 1+n}),
+           ((⤉ syn_inv n N_ClientSpinlock2 (clientSpinlock2_inv n tid2 ℓL ℓl γX γe κs κl γκl γr))
               ∗ (syn_tgt_interp_as n sndl (fun m => (s_memory_black m)))
-              ∗ (isSpinlock n X γX γe κs L)
+              ∗ (⤉ isSpinlock n X γX γe κs ℓL)
               ∗ TID(tid)
-              ∗ (⤉ Duty(tid) [(κl, 0, (∃ κw, (▿ γκl κw)))])
-              ∗ ◇[k](2, 1) ∗ ⤉(live γk (k : nat) (1/2)))
+              ∗ (⤉ Duty(tid) [(κl, 0, (∃ (γκw : τ{nat, n}), ▿ γκl γκw))])
+              ∗ ◇[κl](2, 1)
+              ∗ ◇[κl](2 + ℓL, 1)
+              ∗ (⤉ △ γκl (1/2)))
              -∗
              syn_wpsim (S n) tid ⊤
              (fun rs rt => (⤉(syn_term_cond n tid _ rs rt))%S)
@@ -168,13 +178,91 @@ Section SIM.
              (fn2th ClientSpinlock2Spec.module "thread1" (tt ↑))
              (fn2th ClientSpinlock2.module "thread1" (tt ↑)))%S, 1+n⟧.
   Proof.
-    iIntros. red_tl_all. iIntros (γk). red_tl_all. iIntros (k). red_tl_all. simpl.
-    iEval (rewrite red_syn_inv; rewrite red_syn_wpsim; rewrite red_syn_tgt_interp_as).
+    iIntros.
+    red_tl. iIntros (γX). red_tl. iIntros (γe). red_tl. iIntros (κs).
+    red_tl. iIntros (κl). red_tl. iIntros (γκl). red_tl. iIntros (γr).
+    iEval (red_tl_all; simpl; rewrite red_syn_inv; rewrite red_syn_wpsim; rewrite red_syn_tgt_interp_as).
+    iIntros "(#INV_CL & #MEM & #ISL & TID & DUTY & PC & PC2 & LIVE_l)".
+    unfold fn2th. simpl. unfold thread1, ClientSpinlock2Spec.thread1. rred2r. lred2r.
 
-    iIntros "(#INV & #MEM & THDW & DUTY & PCk & LIVE)".
+    iMod (pc_drop _ 1 _ _ 100 with "PC") as "PC".
+    Unshelve.
+    1,3: lia.
+    iPoseProof (pcs_cons_fold κl 0 [] 1 100 with "[PC]") as "PCS".
+    { iFrame. }
+    iApply (wpsim_yieldR2 with "[DUTY PCS]").
+    3:{ iFrame. iFrame. }
+    1,2: lia.
+    iEval (simpl). iIntros "DUTY _ PCS". rred2r. iApply wpsim_tauR. rred2r.
 
-    unfold fn2th. simpl. unfold thread1, Client01Spec.thread1.
-    rred2r. lred2r.
+    iPoseProof ((Spinlock_lock_spec tid n ⊤) $! X γX γe κs ℓL) as "SPEC".
+    set (P0 := (△ γκl (1/2))%S : sProp n).
+    set (R0 := ((△ γκl (1/2)) ∗ Duty(tid) [(κl, 0, (∃ (γκw : τ{nat, n}), ▿ γκl γκw))])%S : sProp n).
+    set (Q0 := (∃ (κw γκw : τ{nat, n}),
+                   (▿ γκl γκw) ∗ Duty(tid) [(κw, 0, (∃ (γκu : τ{nat}), ▿ γκw γκu))])%S : sProp n).
+    (* iSpecialize ("SPEC" $! [(κl, 0, (∃ (γκw : τ{nat, n}), ▿ γκl γκw)%S)] P0 R0 Q0 2). *)
+    iSpecialize ("SPEC" $! _ P0 R0 Q0 2).
+    iApply ("SPEC" with "[PC2 LIVE_l DUTY] [TID PCS]").
+    (* PRE. *)
+    { Local Opaque env_live_inv.
+      iEval (red_tl_all; simpl).
+      iSplitR. eauto. iSplitR. eauto. iSplitL "LIVE_l".
+      { subst P0. iEval (red_tl_all). iFrame. }
+      iSplitL "DUTY PC2".
+      { iFrame. iApply pcs_cons_fold. iFrame. }
+      iSplitR.
+      - (* ELI. *)
+        Local Transparent env_live_inv.
+        assert (exists a, a = 1). eauto. des. replace 2 with (1 + a) by auto. iEval simpl. subst a.
+        iModIntro. iIntros "FC A". iEval (red_tl_all; simpl; rewrite red_syn_inv) in "A".
+        iDestruct "A" as "(#INV_SL & INV_SL_CLOSE & SL)".
+        iEval (unfold spinlockInv; red_tl_all; simpl) in "SL". iDestruct "SL" as "[(PTX & LX & EX) | (PTX & LX)]".
+        { iModIntro. do 2 iRight. iEval (red_tl_all; simpl; rewrite red_syn_inv). iSplitR. eauto. iFrame. }
+        iInv "INV_CL" as "CL" "INV_CL_CLOSE".
+        iEval (unfold clientSpinlock2_inv; simpl; red_tl_all; simpl) in "CL".
+        iDestruct "CL" as "[CL1 | [CL2 | [CL3 | CL4]]]".
+        + iExFalso. iDestruct "CL1" as "(LXw & _)". iPoseProof (AuthExcls.b_w_eq with "LX LXw") as "%F". inv F.
+        + iDestruct "CL2" as "(LXw & PTD & %κw & CL2)". iEval (red_tl) in "CL2". iDestruct "CL2" as "[%γκw CL2]".
+          iEval (red_tl_all; simpl) in "CL2". iDestruct "CL2" as "(#PROM_w & LIVE_w & #LINK_w & #DEAD_l & PC_spin & DUTY2)".
+          iMod (tpromise_progress with "[FC]") as "[PC_w | #FULF_w]".
+          { iFrame. iApply "PROM_w". }
+          { iMod (link_amplify with "[PC_w]") as "PC_s".
+            { iFrame. iApply "LINK_w". }
+            iMod ("INV_CL_CLOSE" with "[LXw PTD LIVE_w PC_spin DUTY2]") as "_".
+            { iEval (unfold clientSpinlock2_inv; simpl; red_tl_all; simpl). iRight. iLeft. iFrame.
+              iExists _. iEval (red_tl_all). iExists _. iEval (red_tl_all; simpl). iFrame. iSplit. iApply "PROM_w". iSplit; auto.
+            }
+            iModIntro. iLeft. iEval (red_tl; rewrite red_syn_inv). iFrame. iSplitR. auto.
+            iEval (unfold spinlockInv; red_tl_all; simpl). iRight. iFrame.
+          }
+          { iEval (simpl; red_tl_all) in "FULF_w". iDestruct "FULF_w" as "(%γκu & DEAD_w)".
+            iEval (red_tl_all) in "DEAD_w". iPoseProof (OneShots.pending_not_shot with "LIVE_w DEAD_w") as "%F". inv F.
+          }
+        + iDestruct "CL3" as "(LXw & PTD & %γκw & CL3)". iEval (red_tl) in "CL3". iDestruct "CL3" as "[%κu CL3]".
+          iEval (red_tl) in "CL3". iDestruct "CL3" as "[%γκu CL3]".
+          iEval (red_tl_all; simpl) in "CL3". iDestruct "CL3" as "(#PROM_u & LIVE_u & #LINK_u & #DEAD_l & #DEAD_w & PASS)".
+          iMod (tpromise_progress with "[FC]") as "[PC_u | #FULF_u]".
+          { iFrame. iApply "PROM_u". }
+          { iMod (link_amplify with "[PC_u]") as "PC_s".
+            { iFrame. iApply "LINK_u". }
+            iMod ("INV_CL_CLOSE" with "[LXw PTD LIVE_u PASS]") as "_".
+            { iEval (unfold clientSpinlock2_inv; simpl; red_tl_all; simpl). do 2 iRight. iLeft. iFrame.
+              iExists _. iEval (red_tl_all). iExists _. iEval (red_tl_all). iExists _.
+              iEval (red_tl_all; simpl). iFrame. iSplit. iApply "PROM_u". iSplit; eauto.
+            }
+            iModIntro. iLeft. iEval (red_tl; rewrite red_syn_inv). iFrame. iSplitR. auto.
+            iEval (unfold spinlockInv; red_tl_all; simpl). iRight. iFrame.
+          }
+          { iEval (simpl; red_tl_all) in "FULF_u".
+            iPoseProof (OneShots.pending_not_shot with "LIVE_u FULF_u") as "%F". inv F.
+          }
+        + iExFalso. iDestruct "CL4" as "(LXw & _)". iPoseProof (AuthExcls.b_w_eq with "LX LXw") as "%F". inv F.
+
+      -
+        
+          
+
+
 
 
 End SIM.
